\documentclass[11pt, oneside]{article}   	% use "amsart" instead of "article" for AMSLaTeX format
\usepackage{geometry}                		% See geometry.pdf to learn the layout options. There are lots.
\geometry{letterpaper}                   		% ... or a4paper or a5paper or ... 
\usepackage[parfill]{parskip}    		% Activate to begin paragraphs with an empty line rather than an indent
\usepackage{graphicx}				% Use pdf, png, jpg, or epsÂ§ with pdflatex; use eps in DVI mode
								% TeX will automatically convert eps --\rangle pdf in pdflatex		
\usepackage{amssymb}
\usepackage{amsmath}

\usepackage{verbatim}
\usepackage{tikz} 

\usepackage{syntonly}
% \syntaxonly \langle -- use this for checking syntax only
% \mbox {text} - keep together
% \fbox {text} - keep together and draw around

%\pagestyle{plain|headings|empty} % header and footer p.27
%SetFonts
%\include{filename}, \includeonly{filename1, filename2} , \input[fiename}

%SetFonts% 

\title{Brilliant: Vector Calculus}
\author{Dave Fetterman}
\date{6/21/22}							% Activate to display a given date or no date

\begin{document}
\maketitle
Note: Latex reference: http://tug.ctan.org/info/undergradmath/undergradmath.pdf
\section{Chapter 2.1: Calculus of Motion}

Consider vectors of motion against $t$ of the form $ \overrightarrow{x}(t) = \langle x(t), y(t), \ldots \rangle$.
\begin{itemize}
\item A \textbf{line} through $p = (a, b, c)$ parallel to $\overrightarrow{v} = \langle v_x, v_y, v_z\rangle$ is $\overrightarrow{x}(t) = \overrightarrow{p} + t \overrightarrow{v}$ 
\item \textbf{velocity} is characterized completely by $\overrightarrow{v}(t) = \overrightarrow{x}'(t) = \langle x'(t), y'(t), z'(t)\rangle$.
\item The \textbf{speed} of an object along that line versus $t$ is the length of $v$ ($\|v\|$)  
\item Therefore, the speed of an object along line 
$$ \langle x(t), y(t), z(t)\rangle = \langle 0, 2, -3\rangle + t\langle 1,-2,2\rangle$$ is $$\sqrt{1^2+(-2)^2 + 2^2} = 3$$
\item Note that $\overrightarrow{v}$ need not be constant.  The speed of $$\overrightarrow{x}(t) =  \overrightarrow{p} + 3 \sin(2\pi t)\hat{u}, \| \hat{u} \| = 1$$ would then be $$\| 6\pi \cos(2 \pi t) \hat{u} \| = |6\pi \cos(2 \pi t)|$$
\item \textbf{Acceleration} $a(t) = v'(t) = x''(t)$ is straightforward.  Acceleration of $$x(t) = \langle -1 + \cos(t), 1, \cos(t)\rangle = \langle -\cos(t), 0, -\cos(t)\rangle$$
\item An example position vector for a planet of distance $r$ from the sun could be $\langle r \cos(t), r \sin(t) \rangle$.  The acceleration vector points in the opposite direction: $\langle - r \cos(t), - r \sin(t) \rangle$.  In addition to being the analytical second derivative, consider that the \emph{force} of gravity, (which, by $F = ma$ is proportional to acceleration) points towards the sun.  
\item A \textbf{helix} could be a 3D extension like $\langle r \cos(t), r \sin(t), b\cdot t \rangle$.  
\end{itemize}

\section{Chapter 2.2: Space Curves}
\begin{itemize}
\item TODO: Problem 5 - rotating ellipses and solving intersections with planes
\item Note that while $\overrightarrow{x}(t) = \langle \cos(t), \sin(t), 5 \rangle$ and  $\overrightarrow{x}(t) = \langle \cos(2t), \sin(2t), 5 \rangle$ describe the same curve, the space curve also records motion in time, so the \emph{velocity} may be different.
\item If $\overrightarrow{x}(t) = t\overrightarrow{v}$, then speed is $\frac{\| \overrightarrow{x}(t+\Delta t) - \overrightarrow{t} \|}{\Delta t} = \| \overrightarrow{v} \|$,  direction is $\frac{\overrightarrow{v}}{\| \overrightarrow{v} \|}$, and velocity $\overrightarrow{v}$ is the product of speed and direction.
\item So $\overrightarrow{v}(t) = \lim_{\Delta t \rightarrow 0} \frac{\overrightarrow{x}(t + \Delta t) - \overrightarrow{x}(t)}{\Delta t} = \overrightarrow{x}'(t) = \frac{d\overrightarrow{x}}{dt} = \langle x'(t), y'(t), z'(t) \rangle$
\item Neat conceptual result: any $y = f(x)$ can be made into $x(t) = \langle t, f(t), 0 \rangle$, and then $v(t) = \langle 1, f'(t), 0 \rangle$, which points along the tangent line at $\langle t, f(t), 0 \rangle$.
\item Note that dot product derivatives work like regular product: $[\overrightarrow{a}(t) \cdot \overrightarrow{b}(t)]' = \overrightarrow{a}'(t) \cdot \overrightarrow{b}(t) + \overrightarrow{a}(t) \cdot \overrightarrow{b}'(t)$, 
but the cross product does not work the same since $\frac{d}{dt}[a \times b] = a' \times b + a \times b'$, but since $a \times b' = -b' \times a$, can't switch the order to $a' \times b + b' \times a$ due to this non-commutativity.
\item If $$\overrightarrow{x}(t) = \overrightarrow{p}+ t \overrightarrow{v},$$ calculating velocity with respect to origin  becomes
$$ \frac{d}{dt} \| \overrightarrow{x}(t) \| = \frac{\overrightarrow{x}(t) \cdot \overrightarrow{x}'(t)}{\| \overrightarrow{x}(t) \|} = \frac{\overrightarrow{x}}{\| \overrightarrow{x} \|} \cdot \overrightarrow{v},$$ after rewriting the distance formula and chugging through the chain rule.
\item However, it becomes more clear when considering that $(\overrightarrow{v} \cdot \hat{x}) \hat{x}$ is the projection of the velocity vector onto the position vector.  So, the length of this is the rate of change of distance from origin!
\end{itemize}

\section{Chapter 2.3: Integrals and Arc Length}
\begin{itemize}
\item Integral of a vector function can be defined componentwise in a straightforward way: $\int_a^b {\overrightarrow{x}(t)} = \langle \int_a^b {x(t)},  \int_a^b {y(t)},  \int_a^b {z(t)} \rangle $ 
\item Example: if ball launched from origin with velocity $\langle 1, 2, 3 \rangle$ and acceleration $\langle 0, 0, -1 \rangle$, it lands at
\begin{align} 
\frac{dv}{dt}dt = \langle 0, 0, -1 \rangle \\ 
\int{\frac{dv}{dt}dt} = v =  \langle C , D , -t +F \rangle  = \langle 1, 2, 3 \rangle =  \langle 1, 2, -t + 3\rangle, t = 0 \\
x = \int{v}  = \langle t+K, 2t+M, -\frac{1}{2}t^2 + 3t + N \rangle, x(\overrightarrow{0}) = \langle 0 ,0, 0\rangle \\ 
\overrightarrow{x}(t) = \langle t, 2t, 3t-\frac{1}{2}t^2 \rangle \\
z(t) = 0 \rightarrow t = 6 \rightarrow \overrightarrow{x}(6) = \langle 6, 12, 0 \rangle \\
\end{align} 
\item Also, generalizing $ds = \sqrt{(dx)^2  + (dy)^2}$, the length of an arc from point $a$ to $b$ aporoaches $\int_a^b \| x'(t) \| dt$
\item Example: a helix $\langle a \cos (\omega t), a \sin (\omega t), b \omega t \rangle$, parametrized by time $t$ can be rewritten in terms of $s$, the arc length: 
\begin{align}
s =  \int \|x'(t)\| dt \\
s = \int \sqrt{(-\omega a \sin (\omega t))^2 + (\omega a \cos (\omega t))^2 + (b \omega)^2}dt \\
s = |\omega| \int \sqrt{(a^2 + b^2)}dt \\ 
s = |\omega| t \sqrt{a^2 + b^2}
\end{align}
\item \emph{Note: It's weird to think of time in terms of length}.  Could be analytically useful?
\end{itemize}


\section{Chapter 2.4: Frenet Formulae}

Main idea: Establish three new vectors $\hat{T}(s), \hat{N}(s), \hat{B}(s)$ that change as we move along a space curve, instead of $\overrightarrow{x}(t)$ that changes over an external "time" idea.

Remember that  $s = \int_0^t \| \overrightarrow{x}'(\tilde{t}) \| d\tilde{t}$, so $\frac{ds}{dt} = \| \overrightarrow{x}'(t)\|$ .

\subsection{$\hat{T}$: Vector tangent to space curve}
\begin{itemize}
\item Remember arc length is $s = \int_0^t \| \overrightarrow{x}'(\tilde{t})d\tilde{t} \|$
\item $\hat{T}$ is just normalized grad: $\frac{\overrightarrow{x}'(t)}{\|\overrightarrow{x}'(t)\|}$
\item This implies $\frac{d\overrightarrow{x}}{ds} = \hat{T}$ since 
\begin{align}
s = \int_0^t \| \overrightarrow{x}'(\tilde{t})d\tilde{t} \| \\
\frac{ds}{dt} = \| \overrightarrow{x}(t) \| \\
\hat{T} = \frac{\overrightarrow{x}'(t)}{\|\overrightarrow{x}'(t)\|}  = \frac{d\overrightarrow{x}}{dt} \cdot \frac{dt}{ds} \\
\hat{T} = \frac{d\overrightarrow{x}}{ds} \\
\end{align}
\end{itemize}


\subsection{$\hat{N}$: Vector normal to space curve and also in the direction of acceleration}
Normal vectors include
\begin{itemize}
\item $\frac{\hat{T}(t)} { \| \hat{T}(t) \|}$ since, as $\| \hat(T) \| $ is just 1:
\begin{align}
d(\| \hat{T} \|^2) = 0 \\
d(\| \hat{T} \|^2) = d(\hat{T} \cdot \hat{T}) = \hat{T}(t) \cdot 2\hat{T}'(t) \\
\hat{T}(t) \cdot \hat{T}'(t)  = 0
\end{align}
\item $\frac{ \frac{d\hat{T}}{ds}  }  { \| \frac{d\hat{T}}{ds}  \| }$ since it's the same as the above, but parametrized over $s$ instead of $t$.  Doesn't change the direction of the vector!
\end{itemize}

Example:if  $\overrightarrow{x}(t) = \langle R\cos(\omega t), R\sin(\omega t), 0 \rangle$, then acceleration $\overrightarrow{a}(t)$ is
\begin{itemize}
\item $\overrightarrow{a} = \frac{d^2\overrightarrow{x}}{dt^2}$ just by definition
\item $\overrightarrow{a} = -\omega^2 \overrightarrow{x}$ just by calculation
\item $\hat{T}(t) = \langle -\sin(\omega t), \cos (\omega t), 0 \rangle$
\item $\| \hat{T}(t) \| = 1$
\item $\hat{N} = \frac{\hat{T}(t)} { \| \hat{T}(t) \|} =  \langle -cos(\omega t), -\sin (\omega t), 0 \rangle$
\item So $\overrightarrow{a} = R\omega^2\hat{N}$ by these formulae.
\end{itemize}

This leads us to believe acceleration and $\hat{N}$, the normed derivative of $\hat{T}$ are related.

The part of acceleration $\overrightarrow{a}$ parallel to $\hat{T}$ is the projection $(\overrightarrow{a} \cdot \hat{T}) \hat{T}$

The perpendicular part is then $\overrightarrow{a}$ minus that: $\overrightarrow{a} - (\overrightarrow{a} \cdot \hat{T}) \hat{T}$

This also equals $(\frac{ds}{dt})^2 \|\frac{d\hat{T}}{ds} \| \hat{N}$ because
\begin{align}
\overrightarrow{x} = \frac{dx}{dt} = T = \hat{T} \cdot \|  \frac{dx}{dt} \| \\
s = \int_0^t \| \overrightarrow{x}'(t) \rightarrow \frac{ds}{dt} = \| \overrightarrow{x}'(t) \|  \\
\hat{N} = \frac{d\hat{T}}{ds} normalized, so \\
\overrightarrow{a} = \frac{d^2\overrightarrow{x}}{dt^2} = \frac{d}{dt}(\| \overrightarrow{x}'(t)\hat{T}(t)\|) = \frac{d \|\overrightarrow{x}'(t) \|}{dt}\hat{T} + \| \overrightarrow{x}'(t) \| \frac{d\hat{T}}{dt} \\
= \frac{d \|\overrightarrow{x}'(t) \|}{dt}\hat{T} + \frac{ds}{dt} \frac{d\hat{T}}{ds} \frac{ds}{dt} \\ 
= \frac{d \|\overrightarrow{x}'(t) \|}{dt}\hat{T} + (\frac{d{s}}{dt} )^2 \| \frac{d\hat{T}}{ds} \| \hat{N}
\end{align}

This is ``a = parallel part plus perpendicular (N) part'', so the second term is $a_{\bot}$

\subsection{Binormal vector $\hat{B}$}

Note that curvature $\kappa(s) = \| \frac{d\hat{T}}{ds}\|$ is geometric (depends on s, not time) and changes as $\hat{T}$ changes.

Example: Curvature of $\overrightarrow{x}(t) = \langle \cos(t), \sin(t), bt \rangle$ 
\begin{align}
x'(t) = \langle -\sin(t), \cos(t), b \rangle \\ 
\|x'(t) \| = \sqrt(1 + b^2) \\ 
s = \int_0^t\|x'(t)\| = \int_0^t \sqrt{(1+b^2)} = t\sqrt{(1+b^2)} \rightarrow t = \frac{s}{\sqrt{1+b^2}}
\end{align}


\subsection{$\hat{T}$ is:} 
\begin{itemize}
\item $\overrightarrow{x}'(t)$ normalized
\item The tangent vector to the curve
\item The same whether paremetrized by $\hat{T}'(t)$ or $\frac{dx}{ds}$
\end{itemize}

\subsection{$\hat{N}$ is:} 
\begin{itemize}
\item $\overrightarrow{x}''(t)$ normalized as $\frac { \frac{d\hat{T}}{ds} }   {\|  \frac{d\hat{T}}{ds}  \|}  = \hat{N}$
\item The normal vector to the curve
\item $\bot$ to $\hat{T}$ in direction of acceleration.  So a multiple of acceleration vector.
\item The same whether paremetrized by $\hat{T}'(t)$ or $\frac{dx}{ds}$
\end{itemize}

\subsection{$\hat{T}$ and $\hat{N}$}:

\begin{itemize}
\item Form a plane, since first, any normal vector's derivative is perpendicular to the vector
\begin{align}
\frac{d}{ds} \|\hat{T}\|^2 = \frac{d}{ds} \hat{T} \cdot \hat{T} \\
= 2\hat{T} \cdot \hat{T}' \\
\frac{d}{ds} \|\hat{T}\|^2 = \frac{d}{ds} 1 = 0 \\
\end{align}
and 
\begin{align}
\hat{T} \cdot \hat{N} =   \hat{T} \cdot \frac { \frac{d\hat{T}}{ds} }   {\|  \frac{d\hat{T}}{ds}  \|} \\ 
=  \hat{T} \cdot \frac { \hat{T}'(s)}  {\|  \frac{d\hat{T}}{ds}  \|} = 0 
\end{align}
\item $\kappa$ is curvature: how much we're curving in that $T \times N$ plane.
\item $\kappa =   \|  \frac{d\hat{T}}{ds}  \| $ 
\item Therefore, by above, $\frac{d\hat{T}}{ds} = \kappa \hat{N}$ \textbf{(Frenet equation 1)}

\end{itemize}

\subsection{$\hat{B}$ is binormal: perpendicular to both}
\begin{itemize}
\item defined as $\hat{B} = \hat{T} \times \hat{N}$
\item Therefore, by derivative 
\begin{align}
\frac{d\hat{B}}{ds} = \frac{d\hat{T}}{ds} \times \hat{N} +  \hat{T} \times \frac{d\hat{N}}{ds}\\ 
\frac{d\hat{B}}{ds} = \kappa \hat{N} \times \hat{N}  +  \hat{T} \times \frac{d\hat{N}}{ds}\\ 
\frac{d\hat{B}}{ds} =  \hat{T} \times \frac{d\hat{N}}{ds}\\ 
\end{align}
but this means T is orthogonal to dB, and we already know B and dB are orthogonal.
We're working in 3d with the cross product, so dB is parallel to N.
\item Therefore, we define "torsion" $\tau$ so that $- \frac{d\hat{B}}{ds}  = \tau \hat{N}$  \textbf{(Frenet equation 2)}.  Negative sign by convention.
\item Can also cross by $N$ on both sides to get $- \frac{d\hat{B}}{ds}  \times \hat{N} = \tau $ 
\item $\hat{B}$ measures how the plane defined by $\hat{T}, \hat{N}$ twists around.  On a circle, $\hat{B}$ wouldn't change, so the derivative would be zero.
\item \textbf{Final Frenet equation}.  Prereq: $\hat{B} = \hat{T} \times \hat{N} \rightarrow \hat{N} = \hat{B} \times \hat{T} \rightarrow \hat{T} = \hat{N} \times \hat{B}$
\begin{align}
\frac{d\hat{N}}{ds} = \frac{d\hat{B}}{ds} \times \hat{T} +   \hat{B} \times  \frac{d\hat{T}}{ds} \\
\frac{d\hat{N}}{ds} = -\tau \hat{N} \times \hat{T} + \hat{B} \times \kappa \hat{N} \\ 
\frac{d\hat{N}}{ds}  = \tau \hat{B} - \kappa \hat{T}
\end{align}

\end{itemize}

\section{Chapter 2.5: Parametrized Surfaces}

Main ideas:
\begin{itemize}
\item Can parameterize by $\overrightarrow{x}(u,v) = x(u,v), y(u,v), z(u,v)$
\item Can perhaps parameterize $f(x,y,z) = c$ by $z = g(x,y)$
\item Can also use ideas like $\nabla f = 0$ to find a normal.
\end{itemize}

There are many out-of-the-box paremetrizations including:

\begin{itemize}
\item Sphere at 0,0,0: $\overrightarrow{x}(u,v) = \langle R\cos(u)\sin(v), Rsin(u)\sin(v), R\cos(v)\rangle$, where $u \in [0, 2\pi), v \in [0, \pi]$
\item Rotate function $y = f(x)$ around the x-axis: $\overrightarrow{x}(u,v) = \langle u, f(u)\cos(v), f(u)\sin(v) \rangle$, where $u \in D, v \in [0, 2\pi]$
\end{itemize}

Tangent vectors to $\overrightarrow{x}(u,v)$ are $\frac{\delta \overrightarrow{x}} {du}, \frac{\delta \overrightarrow{x}} {dv}$, so unit normal is 	$\pm \frac 
					{\frac{d \overrightarrow{x}} {du} \times \frac{\delta \overrightarrow{x}}{dv}}
					{\| \frac{d \overrightarrow{x}} {du} \times \frac{\delta \overrightarrow{x}}{dv} \|}
					$
					
Example: Torus $\overrightarrow{x} = \langle [2 + \cos(v)]\cos(u),  [2 + \cos(v)]\sin(u), \sin(v)\rangle, u,v \in [0,2 \pi)$.  What's the tangent plane at $u = \frac{\pi}{4}, v=0$?
\begin{align}
dx/du = \langle -\sin(u)(2 + \cos(v)),  \cos(u)(2 + \cos(v)), 0 \rangle \\
dx/dv = \langle -\sin(v)\cos(u), -\sin(v)\sin(u), \cos(v) \rangle \\
u = \frac{\pi}{4}, v=0 \rightarrow dx/du  \\
= -\frac{3}{\sqrt{2}}, \frac{3}{\sqrt{2}}, 0, dx/dv = 0, 0, 1 \\
dx/du \times dx/dv = \langle  \frac{3}{\sqrt{2}}, \frac{3}{\sqrt{2}}, 0\rangle \\
\hat{n} =  \langle \frac{1}{\sqrt{2}}, \frac{1}{\sqrt{2}}, 0 \rangle \\
\hat{n}  \cdot \overrightarrow{x} = 0 \rightarrow \hat{n} \cdot (x - x_0, y-y_0, z-z_0) = 0 \\
\rightarrow ... \rightarrow x + y = 3\sqrt{2}  \\
\end{align}



\subsection{Example: Ellipsoid $x^2 + 2y^2 + z^2 = 4$}
What's the normal at $(1, \frac{1}{\sqrt{2}}, \sqrt{2})$?

\textbf{Method 1: parametrize with spherical u, v}
First, transform to sphere with change of coordinates
\begin{align}
x^2 + 2y^2 + z^2 = 4 \\
X = x/2, Y=\frac{Y}{\sqrt{2}}, Z = z/2 \\
X^2 + Y^2 + Z^2 = 1 \\
X = \cos(u)\sin(v), Y = \sin(u)\sin(v), Z = \cos(v) \\
p = (1, \frac{1}{\sqrt{2}}, \sqrt{2})  \rightarrow u = v = \frac{\pi}{4} \\
\frac{dx}{du}(\frac{\pi}{4}, \frac{\pi}{4}) = \langle -1, \frac{1}{\sqrt{2}}, 0 \rangle \\
\frac{dx}{dv}(\frac{\pi}{4}, \frac{\pi}{4}) = \langle 1, \frac{1}{\sqrt{2}}, -\sqrt{2} \rangle \\
\frac{dx}{du}(\frac{\pi}{4}, \frac{\pi}{4}) \times \frac{dx}{dv}(\frac{\pi}{4}, \frac{\pi}{4}) = \langle 1, \sqrt{2}, \sqrt{2}\rangle \\
\hat{n}_{out} = \frac{\langle -1, -\sqrt{2}, -\sqrt{2}\rangle }{\sqrt{5}}
\end{align}


\textbf{Method 2: rewrite as z = g(x,y)}

\begin{align}
x^2 + 2y^2 + z^2 = 4 \\
z = (4 - x^2 - 2y^2)^\frac{1}{2} \\
dz / dx = \frac{1}{2} \times -2x (4 - x^2 - 2y^2)^{-\frac{1}{2}} = -\frac{1}{\sqrt{2}} \\
dz / dy = \frac{1}{2} \times -4y (4 - x^2 - 2y^2)^{-\frac{1}{2}} =-2\sqrt{2}/\sqrt{2} = -1\\
f \approx \sqrt{2}  + dz / dx(1, \frac{1}{\sqrt{2}})(x - 1) + dz / dy (1,  \frac{1}{\sqrt{2}}) (y - \frac{1}{\sqrt{2}})\\
\rightarrow ... \rightarrow \frac{1}{\sqrt{2}}x + y + z = 2\sqrt{2} \\
\end{align}

giving us normal vector $\langle \frac{1}{\sqrt{2}}, 1, 1 \rangle = \frac{\langle 1, \sqrt{2}, \sqrt{2}\rangle }{\sqrt{5}}$
after normalization.

\textbf{Method 3: gradient}

Gradient is always normal to the tangent plane.
Recognize level set of $f(x,y,z) = x^2 + 2y^2 + z^2$.  

$\nabla f = \langle 2x, 4y, 2z \rangle \rightarrow \nabla f(1, \frac{1}{\sqrt{2}}, \sqrt{2}) = \langle 2, 2\sqrt{2}, 2\sqrt{2}\rangle$

Then normalize.

\subsection{Mobius strip and "direction of out"}
Mobius strip is 
\begin{itemize}
\item $x = 2\cos(u) + v\cos(\frac{u}{2})$
\item $y = 2\sin(u) + v\cos(\frac{u}{2})$
\item $z = v \sin(\frac{u}{2})$
\item $u \in [0, 2\pi], v \in [-\frac{1}{2}, \frac{1}{2}]$
\end{itemize}

$\hat{n} = \frac
	{\overrightarrow{x}_u \times  \overrightarrow{x}_v}
	{\|\overrightarrow{x}_u \times  \overrightarrow{x}_v\|}
	$ at (0,0) is $\langle 0, 0, -1 \rangle$, 
	
but at $(2\pi, 0)$ is the same point, but $\hat{n} = \langle 0, 0, 1 \rangle$!!
	


\section{Chapter 2.6: Vector Fields}

(Lots of intuition questions here...)

One nugget: using \textbf{gradient vector fields}:
Suppose $\overrightarrow{F}(x,y) = \langle 2, -4y^3 \rangle$.  
Then if F = $\nabla f$, then F's arrows are perpendicular to a level set $f = c$.
So look at $f  =  2x -y^4 $ and find perpendicular arrows to these.  That's actually F!

\textbf{Linear approximation for $\overrightarrow{F}: D \in \mathbf{R}^n \rightarrow \mathbf{R}^m$}

Main idea: 
$\overrightarrow{F}(\overrightarrow{x}) = \overrightarrow{F}(\overrightarrow{a}) + A(\overrightarrow{a})(\overrightarrow{x} - \overrightarrow{a})$

Note that $A$ takes in vectors of size $n$ (so it has that many columns), and has $m$ functions (rows) that operate on it.
So the Jacobian, $A$, has as row $i$, column $j$, the quantity $\frac{dF_i}{dx_j}(\overrightarrow{a})$.

$dF_i/d\overrightarrow{x}$ extends across row $i$.

\section{Chapter 2.7: Jack and the Beanstalk (Newton's method)}

\textbf{Basis for Newton's:}

If we're estimating $x_1$ by following the derivative at $x_0$, this means we're looking at the line with x-intercept $x_1$, with slope $f'(x_0)$.

  So instead of $y = mx+b$, we'll flip the two and use 
  
 $x = y/m + x_{int}$ 
 
or $x_0 = f(x_0)\frac{1}{f'(x_0)} + x_1$, 

or $x_1 = x_0 - \frac{f(x_0)}{f'(x_0)}$.

Note that, under Newton's something like $|x|$ will converge immediately, $x^3$ will converge moderately, and a S-curve might barely converge if at all.

The extension of this with the Jacobian matrix $A = DF'(x_0)$ is $\overrightarrow{x}_1 = \overrightarrow{x}_0 - (D\overrightarrow{F}(\overrightarrow{x}_0))^{-1}\overrightarrow{F}(x_0)$ 


\section{Chapter 2.8: Electrostatic bootcamp}

Electric charge radiates out equally in all directions, and is inversely proportional to distance.  

Formula, with $Q$ as the charge, $\epsilon_0$ is a constant: $\overrightarrow{E}(x,y,z) = \frac{Q}{4\pi\epsilon_0\|x\|^2}\hat{x}$

\textbf{Field line} is a special case of a {flow line} - the space cure that follows $\overrightarrow{F}$'s arrows.  The tangent vector to the flow line is $\overrightarrow{F}(\overrightarrow{x}(t))$ (t is not time here), so $\frac{d\overrightarrow{x}}{dt} = \overrightarrow{F}(\overrightarrow{x}(t))$

Example: Vector field $\overrightarrow{F}(x,y) = \langle -2y, 3x \rangle$.  What's the flow line through (2,0)?

Solution: Need to solve 
$dx/dt = -2y, dy/dt = 3x$.  Key is "separating the equations".  Remember x and y are functions of t!

\begin{align}
\frac{d^2x}{dt^2} = -2 \frac{dy}{dt}= -2 \times 3x = -6x.\\
\frac{d^2y}{dt^2} = -2 \frac{dy}{dt}= -2 \times 3x = -6y.\\
x(t) = -6x''(t), y(t) = -6y''(t) \\
\rightarrow x = A\cos(\sqrt{6}t)+ B\sin(\sqrt{6}t),  y = C\cos(\sqrt{6}t)+ D\sin(\sqrt{6}t) \\
\frac{dx}{dt} = -2y(t) \rightarrow   \frac{\sqrt{6}}{2}A\sin(\sqrt{6}t)- \frac{\sqrt{6}}{2}B\cos(\sqrt{6}t)  = y(t) \\
x(t=0) = 2 \rightarrow A = 2 \\
y(t=0) = 0 \rightarrow B = 0 \\
\overrightarrow{F}(t) = \langle 2\cos(\sqrt{6}t), \sqrt{6}\sin(\sqrt{6}t),\rangle \\
\end{align}

Note: \textbf{Field lines} follow rules:
\begin{itemize}
\item Go from positive charges to negative
\item Density of lines directly relates to how much charge a point has
\item Lines don't intersect.
\item Corollary: If count of out equals count of in, point has zero charge
\item "Number" (to be defined) of field lines in and out of a \emph{surface} related to the charge inside.  Upcoming.
\end{itemize}

\section{3.1: Surface Integrals}

Example: Fluid pressure in a tank is:
\begin{itemize}
\item Proportional (via some weight constant $p_{fluid}$) to depth of the point
\item Pushes out via the normal $\hat{n}$ 
\item So, for the x side of a cube of length l, this would be 

$\overrightarrow{F}_{x=l} = (\iint_{[0,l] \times [0,l]} p_{fluid} [1 - \frac{z}{l}] dy dz) \hat{i}$
\end{itemize}

\textbf{Example}: Hemisphere of size l, sitting at (0, 0, 0)

Finding the out pointing unit normal of hemisphere at point $(x, y, -\sqrt{l^2-x^2-y^2})$

Note: Can just eyeball this, but one way is the \textbf{gradient}.  
Take the level set 


\begin{align}
g(x,y,z) = x^2  + y^2 + (z - l)^2 - l^2 = 0 \\
\nabla g(x,y,z) = \langle 2x , 2y , 2(z-l)  \rangle \\
\hat{n} = \pm \frac{\nabla g(x,y,z)}{ \|\nabla g(x,y,z) \|} \\ 
\hat{n} = \pm \frac{\langle x , y , (z-l)  \rangle}{\sqrt{x^2 + y^2 + (z-l)^2}} \\
\hat{n} = \pm \frac{\langle x , y , (z-l) \rangle}{\sqrt{l^2}} \\
\hat{n} = \pm \langle \frac{x}{l}, \frac{y}{l} ,\frac{z}{l} - 1\rangle \\
\end{align}


Note: Integrating over a patch dA on the surface means finding the area of micro-patches 
$\delta A_{ij}$, which is the parallelogram defined by 
\begin{align}
s_1 = \langle \Delta x_i, 0, \Delta x_i f_x(x_i^*,y_j^*) \rangle \\
s_2 = \langle 0, \Delta y_j, \Delta y_j f_y(x_i^*,y_j^*) \rangle \\ 
\Delta A_{ij} \approx \| s_1 \times s_2 \| \\ 
= \sqrt{ (1 + [ f_x(x_i^*,y_j^*)]^2 + [f_y(x_i^*,y_j^*)]^2 }\Delta x_i \Delta y)_j \\ 
\end{align}

So the total pressure ends up being $\overrightarrow{F}_{tot} = p_{fluid} \iint p  \hat{n}  dA$
\end{document}

